kalloc/Verif_basic_allocation.v
@@ -8,8 +8,6 @@ Require Import VC.tactics.
 
 Require Import VC.kalloc.
 
-
-
 Local Open Scope logic.
 
 
@@ -17,20 +15,20 @@ Definition kalloc_write_42_spec : ident * funspec :=
     DECLARE _kalloc_write_42
     WITH sh : share, original_freelist_pointer:val, xx:Z, ls:list val, gv:globals
     PRE [ ] 
-        PROP () PARAMS() GLOBALS(gv) SEP (KF_globals gv sh ls xx original_freelist_pointer)
+        PROP () PARAMS() GLOBALS(gv) SEP (KAF_globals gv sh ls xx original_freelist_pointer)
     POST [ tint ] 
         EX r,
         PROP ( ) RETURN (r) SEP (
             (if eq_dec original_freelist_pointer nullval then
                 (!! (r = Vint (Int.repr 0)) &&
-                KF_globals gv  sh ls xx original_freelist_pointer * emp)
+                KAF_globals gv  sh ls xx original_freelist_pointer * emp)
             else
             EX next ls',
                 (!! (next :: ls' = ls /\
                     r = Vint (Int.repr 42)
                  ) &&
                     data_at sh tint (Vint (Int.repr 42)) original_freelist_pointer *
-                    KF_globals gv  sh ls' xx next
+                    KAF_globals gv  sh ls' xx next
             )
             )
         ).
@@ -41,16 +39,16 @@ Definition kalloc_int_array_spec : ident * funspec :=
     PRE [ tint ] 
     PROP (0 <= n /\ sizeof (tarray tint n) <= PGSIZE) (* make sure an array of size n fits into the page *)
     PARAMS(Vint (Int.repr n)) GLOBALS(gv) 
-    SEP (KF_globals gv sh ls xx original_freelist_pointer)
+    SEP (KAF_globals gv sh ls xx original_freelist_pointer)
     POST [ tptr tint ]
     PROP ( ) RETURN () SEP (
         (if eq_dec original_freelist_pointer nullval then
-            KF_globals gv  sh ls xx original_freelist_pointer * emp
+            KAF_globals gv  sh ls xx original_freelist_pointer * emp
         else
         EX next ls',
             (!! (next :: ls' = ls) &&
                 array_42_rep sh n original_freelist_pointer *
-                KF_globals gv  sh ls' xx next
+                KAF_globals gv  sh ls' xx next
         )
         )
     ).
@@ -59,26 +57,26 @@ Definition kalloc_int_array_spec_fail : ident * funspec :=
     DECLARE _kalloc_int_array
     WITH sh : share, original_freelist_pointer:val, xx:Z, ls:list val, gv:globals, n:Z
     PRE [ tint ] 
-    PROP (0 <= n <= Int.max_signed) PARAMS(Vint (Int.repr n)) GLOBALS(gv) SEP (KF_globals gv sh ls xx original_freelist_pointer)
+    PROP (0 <= n <= Int.max_signed) PARAMS(Vint (Int.repr n)) GLOBALS(gv) SEP (KAF_globals gv sh ls xx original_freelist_pointer)
     POST [ tptr tint ]
     PROP ( ) RETURN () SEP (
         (if eq_dec original_freelist_pointer nullval then
-            KF_globals gv  sh ls xx original_freelist_pointer * emp
+            KAF_globals gv  sh ls xx original_freelist_pointer * emp
         else
         EX next ls',
             (!! (next :: ls' = ls) &&
                 array_42_rep sh n original_freelist_pointer*
-                KF_globals gv  sh ls' xx next
+                KAF_globals gv  sh ls' xx next
         )
         )
     ).
 
-Lemma body_kalloc_write_42: semax_body KFVprog KFGprog f_kalloc_write_42 kalloc_write_42_spec.
+Lemma body_kalloc_write_42: semax_body KAFVprog KAFGprog f_kalloc_write_42 kalloc_write_42_spec.
 Proof.
 start_function.
 forward. 
-forward_call (kalloc_spec_sub KF_APD tint) (gv, sh , ls, xx, original_freelist_pointer ). (* kalloc *)
-- unfold KF_globals. entailer!.
+forward_call (kalloc_spec_sub KAF_APD tint) (gv, sh , ls, xx, original_freelist_pointer ). (* kalloc *)
+- unfold KAF_globals. entailer!.
 - if_tac.
     + forward_if.
         * rewrite H in H0; auto_contradict.
@@ -93,12 +91,12 @@ forward_call (kalloc_spec_sub KF_APD tint) (gv, sh , ls, xx, original_freelist_p
         * forward.
 Qed.
 
-Lemma body_kalloc_int_array: semax_body KFVprog KFGprog f_kalloc_int_array kalloc_int_array_spec.
+Lemma body_kalloc_int_array: semax_body KAFVprog KAFGprog f_kalloc_int_array kalloc_int_array_spec.
 Proof.
 start_function.
 forward.
-forward_call (kalloc_spec_sub KF_APD (tarray tint n)) (gv, sh , ls, xx, original_freelist_pointer ). (* kalloc *)
-- unfold KF_globals. entailer!.
+forward_call (kalloc_spec_sub KAF_APD (tarray tint n)) (gv, sh , ls, xx, original_freelist_pointer ). (* kalloc *)
+- unfold KAF_globals. entailer!.
 - destruct H; auto.
 - if_tac.
     + forward_if.
@@ -119,7 +117,7 @@ forward_call (kalloc_spec_sub KF_APD (tarray tint n)) (gv, sh , ls, xx, original
         SEP (
             (
                 tmp_array_42_rep sh n original_freelist_pointer i*
-                KF_globals gv sh ls xx v
+                KAF_globals gv sh ls xx v
             )
             )
         )%assert.
@@ -127,7 +125,7 @@ forward_call (kalloc_spec_sub KF_APD (tarray tint n)) (gv, sh , ls, xx, original
         assert (Z.max 0 n <= PGSIZE / (sizeof tint)). {  apply Zdiv_le_lower_bound. simpl; try rep_lia. auto. rewrite Z.mul_comm. auto. }
         assert (n <= PGSIZE / (sizeof tint)); try rep_lia. apply (Z.le_trans) with (PGSIZE / sizeof tint). try rep_lia.
         unfold PGSIZE; simpl; try rep_lia.
-        -- entailer!. unfold tmp_array_42_rep. unfold KF_globals. entailer!. inversion H1; entailer.
+        -- entailer!. unfold tmp_array_42_rep. unfold KAF_globals. entailer!. inversion H1; entailer.
         -- Intros.
         assert (Int.min_signed <= i <= Int.max_signed). { 
             assert (n <= Int.max_signed). {
@@ -174,12 +172,12 @@ forward_call (kalloc_spec_sub KF_APD (tarray tint n)) (gv, sh , ls, xx, original
     * forward.
 Qed.
 
-Lemma body_kalloc_int_array_fail: semax_body KFVprog KFGprog f_kalloc_int_array kalloc_int_array_spec_fail.
+Lemma body_kalloc_int_array_fail: semax_body KAFVprog KAFGprog f_kalloc_int_array kalloc_int_array_spec_fail.
 Proof.
 start_function.
 forward.
-forward_call (kalloc_spec_sub KF_APD (tarray tint n)) (gv, sh , ls, xx, original_freelist_pointer ). (* kalloc *)
-- unfold KF_globals. entailer!.
+forward_call (kalloc_spec_sub KAF_APD (tarray tint n)) (gv, sh , ls, xx, original_freelist_pointer ). (* kalloc *)
+- unfold KAF_globals. entailer!.
 - assert (exists n : Z, sizeof (tarray tint n) > PGSIZE). 
     {
         exists PGSIZE.
