kalloc/Verif_tests_alloc_and_dealloc.v
@@ -19,9 +19,9 @@ Definition kfree_kalloc_spec :=
         PROP(is_pointer_or_null new_head) 
         PARAMS (new_head) GLOBALS(gv)
         SEP (
-            KF_globals gv  sh ls xx original_freelist_pointer *
+            KAF_globals gv  sh ls xx original_freelist_pointer *
             (if eq_dec new_head nullval then emp
-            else (kalloc_token' KF_APD sh (sizeof t_run) new_head))
+            else (kalloc_token' KAF_APD sh (sizeof t_run) new_head))
         )
     POST [ tptr tvoid ]
         EX r,
@@ -34,17 +34,17 @@ Definition kfree_kalloc_spec :=
         SEP (
             let freelist_case :=
             if eq_dec original_freelist_pointer nullval then
-            emp * KF_globals gv sh ls xx original_freelist_pointer
+            emp * KAF_globals gv sh ls xx original_freelist_pointer
             else
             EX next, EX ls',
                 !! (next :: ls' = ls) &&
-                KF_globals gv sh ls' xx next *
-                kalloc_token' KF_APD sh (sizeof t_run) original_freelist_pointer
+                KAF_globals gv sh ls' xx next *
+                kalloc_token' KAF_APD sh (sizeof t_run) original_freelist_pointer
         in
         
         let newhead_case :=
-            KF_globals gv sh ls xx original_freelist_pointer *
-            kalloc_token' KF_APD sh (sizeof t_run) new_head
+            KAF_globals gv sh ls xx original_freelist_pointer *
+            kalloc_token' KAF_APD sh (sizeof t_run) new_head
         in
         
         if eq_dec new_head nullval then
@@ -58,16 +58,16 @@ Definition kalloc_write_42_kfree_spec : ident * funspec :=
     DECLARE _kalloc_write_42_kfree
     WITH sh : share, original_freelist_pointer:val, xx:Z, ls:list val, gv:globals
     PRE [ ] 
-        PROP () PARAMS() GLOBALS(gv) SEP (KF_globals gv sh ls xx original_freelist_pointer)
+        PROP () PARAMS() GLOBALS(gv) SEP (KAF_globals gv sh ls xx original_freelist_pointer)
     POST [ tint ] 
         EX r,
         PROP ( ) RETURN (r) SEP (
             (if eq_dec original_freelist_pointer nullval then
                 (!! (r = Vint (Int.repr 0)) &&
-                KF_globals gv  sh ls xx original_freelist_pointer)
+                KAF_globals gv  sh ls xx original_freelist_pointer)
             else
                 (!! ( r = Vint (Int.repr 42) ) &&
-                KF_globals gv  sh ls xx original_freelist_pointer)
+                KAF_globals gv  sh ls xx original_freelist_pointer)
             )
         ).
         
@@ -81,11 +81,11 @@ Definition kfree_kalloc_twice_spec:=
         ) 
         PARAMS (pa1; pa2) GLOBALS(gv)
         SEP (
-            KF_globals gv  sh ls xx original_freelist_pointer *
+            KAF_globals gv  sh ls xx original_freelist_pointer *
             (if eq_dec pa1 nullval then emp
-            else (kalloc_token' KF_APD sh (sizeof t_run) pa1)) *
+            else (kalloc_token' KAF_APD sh (sizeof t_run) pa1)) *
             (if eq_dec pa2 nullval then emp
-            else (kalloc_token' KF_APD sh (sizeof t_run) pa2))
+            else (kalloc_token' KAF_APD sh (sizeof t_run) pa2))
         )
     POST [ tptr tvoid ]
         EX r,
@@ -101,45 +101,45 @@ Definition kfree_kalloc_twice_spec:=
             SEP 
             (
                 let freelist_only_pa1_null_case :=
-                kalloc_token' KF_APD sh (sizeof t_run) pa2 *
+                kalloc_token' KAF_APD sh (sizeof t_run) pa2 *
                 (if eq_dec original_freelist_pointer nullval then
-                    KF_globals gv sh ls xx original_freelist_pointer * emp
+                    KAF_globals gv sh ls xx original_freelist_pointer * emp
                 else
                     EX next, EX ls',
                     !! (next :: ls' = ls) &&
-                    KF_globals gv sh ls' xx next *
-                    kalloc_token' KF_APD sh (sizeof t_run) original_freelist_pointer)
+                    KAF_globals gv sh ls' xx next *
+                    kalloc_token' KAF_APD sh (sizeof t_run) original_freelist_pointer)
                 in
                 let freelist_only_pa2_null_case :=
-                    kalloc_token' KF_APD sh (sizeof t_run) pa1 * 
+                    kalloc_token' KAF_APD sh (sizeof t_run) pa1 * 
                     (if eq_dec original_freelist_pointer nullval then 
-                        KF_globals gv sh ls xx original_freelist_pointer * emp
+                        KAF_globals gv sh ls xx original_freelist_pointer * emp
                     else 
                         (EX next, EX ls',
                         !! (next :: ls' = ls) &&
-                        KF_globals gv sh ls' xx next *
-                        kalloc_token' KF_APD sh (sizeof t_run) original_freelist_pointer) ) 
+                        KAF_globals gv sh ls' xx next *
+                        kalloc_token' KAF_APD sh (sizeof t_run) original_freelist_pointer) ) 
                 in
                 let freelist_both_null_case :=
                     if eq_dec original_freelist_pointer nullval then
-                        emp * KF_globals gv sh ls xx original_freelist_pointer
+                        emp * KAF_globals gv sh ls xx original_freelist_pointer
                     else
-                        (kalloc_token' KF_APD sh (sizeof t_run) original_freelist_pointer *
+                        (kalloc_token' KAF_APD sh (sizeof t_run) original_freelist_pointer *
                         (EX next1, EX ls1,
                         !! (next1:: ls1 = ls) &&
                         if eq_dec next1 nullval then
-                            KF_globals gv sh ls1 xx next1
+                            KAF_globals gv sh ls1 xx next1
                         else (
                         EX next2, EX ls2,
                         !! (next2:: ls2 = ls1) &&
-                        KF_globals gv sh ls2 xx next2 * 
-                        kalloc_token' KF_APD sh (sizeof t_run) next1
+                        KAF_globals gv sh ls2 xx next2 * 
+                        kalloc_token' KAF_APD sh (sizeof t_run) next1
                         )))
                 in
                 let both_pointers_case :=
-                KF_globals gv sh ls xx original_freelist_pointer *
-                kalloc_token' KF_APD sh (sizeof t_run) pa1 *
-                kalloc_token' KF_APD sh (sizeof t_run) pa2
+                KAF_globals gv sh ls xx original_freelist_pointer *
+                kalloc_token' KAF_APD sh (sizeof t_run) pa1 *
+                kalloc_token' KAF_APD sh (sizeof t_run) pa2
                 in
                 if eq_dec pa1 nullval then
                     if eq_dec pa2 nullval then
@@ -162,11 +162,11 @@ Definition kfree_kalloc_kfree_kalloc_spec:=
         ) 
         PARAMS (pa1; pa2) GLOBALS(gv)
         SEP (
-            KF_globals gv  sh ls xx original_freelist_pointer *
+            KAF_globals gv  sh ls xx original_freelist_pointer *
             (if eq_dec pa1 nullval then emp
-            else (kalloc_token' KF_APD sh (sizeof t_run) pa1)) *
+            else (kalloc_token' KAF_APD sh (sizeof t_run) pa1)) *
             (if eq_dec pa2 nullval then emp
-            else (kalloc_token' KF_APD sh (sizeof t_run) pa2))
+            else (kalloc_token' KAF_APD sh (sizeof t_run) pa2))
         )
     POST [ tptr tvoid ]
         EX r,
@@ -182,45 +182,45 @@ Definition kfree_kalloc_kfree_kalloc_spec:=
             SEP 
             (
                 let freelist_only_pa1_null_case :=
-                kalloc_token' KF_APD sh (sizeof t_run) pa2 *
+                kalloc_token' KAF_APD sh (sizeof t_run) pa2 *
                 (if eq_dec original_freelist_pointer nullval then
-                    KF_globals gv sh ls xx original_freelist_pointer * emp
+                    KAF_globals gv sh ls xx original_freelist_pointer * emp
                 else
                     EX next, EX ls',
                     !! (next :: ls' = ls) &&
-                    KF_globals gv sh ls' xx next *
-                    kalloc_token' KF_APD sh (sizeof t_run) original_freelist_pointer)
+                    KAF_globals gv sh ls' xx next *
+                    kalloc_token' KAF_APD sh (sizeof t_run) original_freelist_pointer)
                 in
                 let freelist_only_pa2_null_case :=
-                    kalloc_token' KF_APD sh (sizeof t_run) pa1 * 
+                    kalloc_token' KAF_APD sh (sizeof t_run) pa1 * 
                     (if eq_dec original_freelist_pointer nullval then 
-                        KF_globals gv sh ls xx original_freelist_pointer * emp
+                        KAF_globals gv sh ls xx original_freelist_pointer * emp
                     else 
                         (EX next, EX ls',
                         !! (next :: ls' = ls) &&
-                        KF_globals gv sh ls' xx next *
-                        kalloc_token' KF_APD sh (sizeof t_run) original_freelist_pointer) ) 
+                        KAF_globals gv sh ls' xx next *
+                        kalloc_token' KAF_APD sh (sizeof t_run) original_freelist_pointer) ) 
                 in
                 let freelist_both_null_case :=
                     if eq_dec original_freelist_pointer nullval then
-                        emp * KF_globals gv sh ls xx original_freelist_pointer
+                        emp * KAF_globals gv sh ls xx original_freelist_pointer
                     else
-                        (kalloc_token' KF_APD sh (sizeof t_run) original_freelist_pointer *
+                        (kalloc_token' KAF_APD sh (sizeof t_run) original_freelist_pointer *
                         (EX next1, EX ls1,
                         !! (next1:: ls1 = ls) &&
                         if eq_dec next1 nullval then
-                            KF_globals gv sh ls1 xx next1
+                            KAF_globals gv sh ls1 xx next1
                         else (
                         EX next2, EX ls2,
                         !! (next2:: ls2 = ls1) &&
-                        KF_globals gv sh ls2 xx next2 * 
-                        kalloc_token' KF_APD sh (sizeof t_run) next1
+                        KAF_globals gv sh ls2 xx next2 * 
+                        kalloc_token' KAF_APD sh (sizeof t_run) next1
                         )))
                 in
                 let both_pointers_case :=
-                KF_globals gv sh ls xx original_freelist_pointer *
-                kalloc_token' KF_APD sh (sizeof t_run) pa1 *
-                kalloc_token' KF_APD sh (sizeof t_run) pa2
+                KAF_globals gv sh ls xx original_freelist_pointer *
+                kalloc_token' KAF_APD sh (sizeof t_run) pa1 *
+                kalloc_token' KAF_APD sh (sizeof t_run) pa2
                 in
                 if eq_dec pa1 nullval then
                     if eq_dec pa2 nullval then
@@ -242,11 +242,11 @@ Definition kfree_kfree_kalloc_spec :=
         ) 
         PARAMS (pa1; pa2) GLOBALS(gv)
         SEP (
-            KF_globals gv  sh ls xx original_freelist_pointer *
+            KAF_globals gv  sh ls xx original_freelist_pointer *
             (if eq_dec pa1 nullval then emp
-            else (kalloc_token' KF_APD sh (sizeof t_run) pa1)) *
+            else (kalloc_token' KAF_APD sh (sizeof t_run) pa1)) *
             (if eq_dec pa2 nullval then emp
-            else (kalloc_token' KF_APD sh (sizeof t_run) pa2))
+            else (kalloc_token' KAF_APD sh (sizeof t_run) pa2))
         )
     POST [ tptr tvoid ]
         EX r,
@@ -260,26 +260,26 @@ Definition kfree_kfree_kalloc_spec :=
         SEP 
         (
             let freelist_only_pa1_null_case :=
-                kalloc_token' KF_APD sh (sizeof t_run) pa2 *
-                KF_globals gv sh ls xx original_freelist_pointer
+                kalloc_token' KAF_APD sh (sizeof t_run) pa2 *
+                KAF_globals gv sh ls xx original_freelist_pointer
             in
             let freelist_only_pa2_null_case :=
-                kalloc_token' KF_APD sh (sizeof t_run) pa1 * 
-                KF_globals gv sh ls xx original_freelist_pointer
+                kalloc_token' KAF_APD sh (sizeof t_run) pa1 * 
+                KAF_globals gv sh ls xx original_freelist_pointer
             in
             let freelist_both_null_case :=
                 if eq_dec original_freelist_pointer nullval then
-                    emp * KF_globals gv sh ls xx original_freelist_pointer
+                    emp * KAF_globals gv sh ls xx original_freelist_pointer
                 else
                     (EX next, EX ls',
                     !! (next :: ls' = ls) &&
-                    KF_globals gv sh ls' xx next *
-                    kalloc_token' KF_APD sh (sizeof t_run) original_freelist_pointer)
+                    KAF_globals gv sh ls' xx next *
+                    kalloc_token' KAF_APD sh (sizeof t_run) original_freelist_pointer)
             in
             let both_is_pointers_case :=
-                KF_globals gv sh (original_freelist_pointer::ls) xx pa1 *
-                (*kalloc_token' KF_APD sh (sizeof t_run) pa1 *)
-                kalloc_token' KF_APD sh (sizeof t_run) pa2
+                KAF_globals gv sh (original_freelist_pointer::ls) xx pa1 *
+                (*kalloc_token' KAF_APD sh (sizeof t_run) pa1 *)
+                kalloc_token' KAF_APD sh (sizeof t_run) pa2
             in
             if eq_dec pa1 nullval then
                 if eq_dec pa2 nullval then
@@ -297,16 +297,16 @@ Definition kalloc_write_42_kfree_kfree_spec : ident * funspec :=
     DECLARE _kalloc_write_42_kfree_kfree
     WITH sh : share, original_freelist_pointer:val, xx:Z, ls:list val, gv:globals
     PRE [ ] 
-        PROP () PARAMS() GLOBALS(gv) SEP (KF_globals gv sh ls xx original_freelist_pointer)
+        PROP () PARAMS() GLOBALS(gv) SEP (KAF_globals gv sh ls xx original_freelist_pointer)
     POST [ tint ] 
         EX r,
         PROP ( ) RETURN (r) SEP (
             (if eq_dec original_freelist_pointer nullval then
                 (!! (r = Vint (Int.repr 0)) &&
-                KF_globals gv  sh ls xx original_freelist_pointer)
+                KAF_globals gv  sh ls xx original_freelist_pointer)
             else
                 (!! ( r = Vint (Int.repr 42) ) &&
-                KF_globals gv  sh ls xx original_freelist_pointer)
+                KAF_globals gv  sh ls xx original_freelist_pointer)
             )
         ).
 
@@ -320,22 +320,42 @@ Definition kfree_kfree_kalloc_kalloc_spec :=
         ) 
         PARAMS (pa1; pa2) GLOBALS(gv)
         SEP (
-            KF_globals gv  sh ls xx original_freelist_pointer *
-            kalloc_token' KF_APD sh (sizeof t_run) pa1 *
-            kalloc_token' KF_APD sh (sizeof t_run) pa2
+            KAF_globals gv  sh ls xx original_freelist_pointer *
+            kalloc_token' KAF_APD sh (sizeof t_run) pa1 *
+            kalloc_token' KAF_APD sh (sizeof t_run) pa2
         )
     POST [ tptr tvoid ]
         PROP( )
             RETURN (pa1) (* we return the head like in the pop function*)
             SEP 
             (
-                KF_globals gv  sh ls xx original_freelist_pointer *
-                kalloc_token' KF_APD sh (sizeof t_run) pa1 *
-                kalloc_token' KF_APD sh (sizeof t_run) pa2
+                KAF_globals gv  sh ls xx original_freelist_pointer *
+                kalloc_token' KAF_APD sh (sizeof t_run) pa1 *
+                kalloc_token' KAF_APD sh (sizeof t_run) pa2
                 ).
 
+Definition kfree_kfree_same_pointer_wrong_spec := 
+    DECLARE _kfree_kfree_same_pointer
+    WITH sh : share, pa1:val, original_freelist_pointer:val, xx:Z, gv:globals, ls : list val, next:val
+    PRE [ tptr tvoid ]
+        PROP(
+            isptr pa1
+        ) 
+        PARAMS (pa1) GLOBALS(gv)
+        SEP (
+            KAF_globals gv  sh ls xx original_freelist_pointer *
+            kalloc_token' KAF_APD sh (sizeof t_run) pa1 *
+            kalloc_token' KAF_APD sh (sizeof t_run) pa1
+            )
+    POST [ tvoid ]
+        PROP( )
+            RETURN () (* we return the head like in the pop function*)
+            SEP 
+            (
+                KAF_globals gv  sh (pa1::original_freelist_pointer::ls) xx pa1
+            ).
 
-Definition KFGprog_clients: funspecs := KFGprog ++ [kfree_kalloc_spec].
+Definition KAFGprog_clients: funspecs := KAFGprog ++ [kfree_kalloc_spec].
 
 Ltac simplify_kalloc_token :=
     repeat (
@@ -344,37 +364,37 @@ Ltac simplify_kalloc_token :=
     );
 entailer!.
 
-Lemma body_kfree_kalloc: semax_body KFVprog KFGprog f_kfree_kalloc kfree_kalloc_spec.
+Lemma body_kfree_kalloc: semax_body KAFVprog KAFGprog f_kfree_kalloc kfree_kalloc_spec.
 Proof.
 start_function.
-forward_call (kfree_spec_sub KF_APD t_run) (new_head, gv, sh , ls, xx, original_freelist_pointer). (* call kfree *)
+forward_call (kfree_spec_sub KAF_APD t_run) (new_head, gv, sh , ls, xx, original_freelist_pointer). (* call kfree *)
     + destruct (eq_dec new_head nullval).
-        *unfold KF_globals. entailer!.
-        * unfold KF_globals. entailer!. 
+        *unfold KAF_globals. entailer!.
+        * unfold KAF_globals. entailer!. 
             simplify_kalloc_token. 
     + destruct (eq_dec new_head nullval).
-        *forward_call (kalloc_spec_sub KF_APD t_run) (gv, sh , ls, xx, original_freelist_pointer ). (* kalloc *)
+        *forward_call (kalloc_spec_sub KAF_APD t_run) (gv, sh , ls, xx, original_freelist_pointer ). (* kalloc *)
         destruct (eq_dec original_freelist_pointer nullval).
-            -- forward. Exists nullval. unfold KF_globals. entailer!.
+            -- forward. Exists nullval. unfold KAF_globals. entailer!.
             -- destruct ls.
                 ++ forward. auto_contradict.
                 ++ forward. Exists original_freelist_pointer. entailer. Exists v. entailer.
-                    Exists ls. entailer. unfold KF_globals. entailer!. inversion H0; subst. entailer!.
+                    Exists ls. entailer. unfold KAF_globals. entailer!. inversion H0; subst. entailer!.
                     simplify_kalloc_token. 
-        *forward_call (kalloc_spec_sub KF_APD t_run) (gv, sh, original_freelist_pointer::ls, xx, new_head ). (* kalloc *)
+        *forward_call (kalloc_spec_sub KAF_APD t_run) (gv, sh, original_freelist_pointer::ls, xx, new_head ). (* kalloc *)
         destruct (eq_dec new_head nullval).
             -- forward.
-            -- forward. Exists new_head. entailer. inversion H0; subst; entailer. unfold KF_globals. entailer!. simplify_kalloc_token.
+            -- forward. Exists new_head. entailer. inversion H0; subst; entailer. unfold KAF_globals. entailer!. simplify_kalloc_token.
         Qed.
         
         
         
-Lemma body_kalloc_write_42_kfree: semax_body KFVprog KFGprog f_kalloc_write_42_kfree kalloc_write_42_kfree_spec.
+Lemma body_kalloc_write_42_kfree: semax_body KAFVprog KAFGprog f_kalloc_write_42_kfree kalloc_write_42_kfree_spec.
 Proof.
     start_function.
     forward. 
-    forward_call (kalloc_spec_sub KF_APD tint) (gv, sh , ls, xx, original_freelist_pointer ). (* kalloc *)
-    - unfold KF_globals. entailer!.
+    forward_call (kalloc_spec_sub KAF_APD tint) (gv, sh , ls, xx, original_freelist_pointer ). (* kalloc *)
+    - unfold KAF_globals. entailer!.
     - if_tac.
     + forward_if.
         * rewrite H in H0; auto_contradict.
@@ -385,19 +405,19 @@ Proof.
         * unfold type_kalloc_token. rewrite kalloc_token_sz_split. Intros.
         rewrite memory_block_data_at_; auto. rewrite data_at__eq. Intros. forward.
         forward. 
-        forward_call (kfree_spec_sub KF_APD tint) (original_freelist_pointer, gv, sh , snd ab, xx, (fst ab)). (* call kfree *)
+        forward_call (kfree_spec_sub KAF_APD tint) (original_freelist_pointer, gv, sh , snd ab, xx, (fst ab)). (* call kfree *)
         -- if_tac_auto_contradict.
             unfold type_kalloc_token. rewrite kalloc_token_sz_split. entailer!.
             sep_apply data_at_memory_block. entailer!.
         -- if_tac_auto_contradict.
             forward. Exists (Vint (Int.repr 42)).
-            unfold KF_globals.
+            unfold KAF_globals.
             inversion H0. rewrite H8; rewrite H9.
             entailer!.
         * forward.
         Qed.
         
-Lemma body_kfree_kalloc_twice: semax_body KFVprog KFGprog_clients f_kfree_kalloc_twice kfree_kalloc_twice_spec.
+Lemma body_kfree_kalloc_twice: semax_body KAFVprog KAFGprog_clients f_kfree_kalloc_twice kfree_kalloc_twice_spec.
 Proof.
 start_function. destruct H.
 forward_call (gv, sh, pa1, original_freelist_pointer, xx, ls).
@@ -466,135 +486,135 @@ forward_call (gv, sh, pa1, original_freelist_pointer, xx, ls).
         Qed.
         
         
-Lemma body_kfree_kalloc_kfree_kalloc: semax_body KFVprog KFGprog f_kfree_kalloc_kfree_kalloc kfree_kalloc_kfree_kalloc_spec.
+Lemma body_kfree_kalloc_kfree_kalloc: semax_body KAFVprog KAFGprog f_kfree_kalloc_kfree_kalloc kfree_kalloc_kfree_kalloc_spec.
 Proof.
 start_function. Intros.
 if_tac; if_tac; destruct H; 
-forward_call (kfree_spec_sub KF_APD t_run) (pa1, gv, sh , ls, xx, original_freelist_pointer). (* call kfree *)
-- if_tac_auto_contradict. unfold KF_globals. entailer!.
-- forward_call (kalloc_spec_sub KF_APD t_run) (gv, sh , ls, xx, original_freelist_pointer). (* kalloc *)
+forward_call (kfree_spec_sub KAF_APD t_run) (pa1, gv, sh , ls, xx, original_freelist_pointer). (* call kfree *)
+- if_tac_auto_contradict. unfold KAF_globals. entailer!.
+- forward_call (kalloc_spec_sub KAF_APD t_run) (gv, sh , ls, xx, original_freelist_pointer). (* kalloc *)
     + if_tac_auto_contradict. entailer!.
     + if_tac_auto_contradict. 
-        * forward_call (kfree_spec_sub KF_APD t_run) (pa2, gv, sh , ls, xx, original_freelist_pointer). (* call kfree *)
+        * forward_call (kfree_spec_sub KAF_APD t_run) (pa2, gv, sh , ls, xx, original_freelist_pointer). (* call kfree *)
             -- if_tac_auto_contradict. entailer!.
-            -- if_tac_auto_contradict. forward_call (kalloc_spec_sub KF_APD t_run) (gv, sh , ls, xx, original_freelist_pointer). (* kalloc *)
+            -- if_tac_auto_contradict. forward_call (kalloc_spec_sub KAF_APD t_run) (gv, sh , ls, xx, original_freelist_pointer). (* kalloc *)
                 if_tac.
-                    ++ forward. Exists nullval; unfold KF_globals. entailer!.
+                    ++ forward. Exists nullval; unfold KAF_globals. entailer!.
                     ++ Intros ab. destruct ls; auto_contradict.
         * Intros ab. destruct ls; auto_contradict. 
-        forward_call (kfree_spec_sub KF_APD t_run) (pa2, gv, sh , snd ab, xx, fst ab). (* call kfree *)
+        forward_call (kfree_spec_sub KAF_APD t_run) (pa2, gv, sh , snd ab, xx, fst ab). (* call kfree *)
             -- entailer!.
-            -- if_tac_auto_contradict. forward_call (kalloc_spec_sub KF_APD t_run) (gv, sh , snd ab, xx, fst ab). (* kalloc *)
+            -- if_tac_auto_contradict. forward_call (kalloc_spec_sub KAF_APD t_run) (gv, sh , snd ab, xx, fst ab). (* kalloc *)
                 if_tac.
                     ++ forward. Exists (fst ab) (fst ab) (snd ab). if_tac.
-                        ** unfold KF_globals. unfold type_kalloc_token. entailer!. repeat right. split; auto.
+                        ** unfold KAF_globals. unfold type_kalloc_token. entailer!. repeat right. split; auto.
                         ** entailer.
                     ++ Intros ab0. forward. Exists (fst ab). unfold type_kalloc_token. rewrite mem_mgr_split. 
                         Exists (fst ab) (snd ab). if_tac_auto_contradict. Exists (fst ab0) (snd ab0). rewrite mem_mgr_split; entailer!.
                         repeat right; split; auto.
--if_tac_auto_contradict. unfold KF_globals. entailer!.
-- forward_call (kalloc_spec_sub KF_APD t_run) (gv, sh , ls, xx, original_freelist_pointer). (* kalloc *)
+-if_tac_auto_contradict. unfold KAF_globals. entailer!.
+- forward_call (kalloc_spec_sub KAF_APD t_run) (gv, sh , ls, xx, original_freelist_pointer). (* kalloc *)
 + if_tac_auto_contradict. entailer!.
 + if_tac_auto_contradict. 
-    * forward_call (kfree_spec_sub KF_APD t_run) (pa2, gv, sh , ls, xx, original_freelist_pointer). (* call kfree *)
+    * forward_call (kfree_spec_sub KAF_APD t_run) (pa2, gv, sh , ls, xx, original_freelist_pointer). (* call kfree *)
         -- if_tac_auto_contradict. unfold type_kalloc_token. entailer!.
-        -- if_tac_auto_contradict. forward_call (kalloc_spec_sub KF_APD t_run) (gv, sh , (original_freelist_pointer :: ls), xx, pa2). (* kalloc *)
+        -- if_tac_auto_contradict. forward_call (kalloc_spec_sub KAF_APD t_run) (gv, sh , (original_freelist_pointer :: ls), xx, pa2). (* kalloc *)
             if_tac.
                 ++ forward.
                 ++ Intros ab. destruct ls; auto_contradict;
-                    forward; unfold type_kalloc_token, KF_globals; inversion H6; rewrite H3; rewrite H9; Exists pa2; entailer!;
+                    forward; unfold type_kalloc_token, KAF_globals; inversion H6; rewrite H3; rewrite H9; Exists pa2; entailer!;
                     do 4 right; left; split; auto.
     * Intros ab. destruct ls; auto_contradict.  
-    forward_call (kfree_spec_sub KF_APD t_run) (pa2, gv, sh , snd ab, xx, fst ab). (* call kfree *)
+    forward_call (kfree_spec_sub KAF_APD t_run) (pa2, gv, sh , snd ab, xx, fst ab). (* call kfree *)
         -- if_tac_auto_contradict. unfold type_kalloc_token at 2. rewrite kalloc_token_sz_split. entailer!.
-        -- if_tac_auto_contradict. rewrite mem_mgr_split. Intros. forward_call (kalloc_spec_sub KF_APD t_run) (gv, sh , fst ab::snd ab, xx, pa2). (* kalloc *)
+        -- if_tac_auto_contradict. rewrite mem_mgr_split. Intros. forward_call (kalloc_spec_sub KAF_APD t_run) (gv, sh , fst ab::snd ab, xx, pa2). (* kalloc *)
             ++ unfold type_kalloc_token. rewrite mem_mgr_split.  entailer!.
-            ++ forward. if_tac_auto_contradict. Intros ab0. Exists pa2 (fst ab0) (snd ab0). rewrite mem_mgr_split. unfold KF_globals, type_kalloc_token. rewrite mem_mgr_split. entailer!.
+            ++ forward. if_tac_auto_contradict. Intros ab0. Exists pa2 (fst ab0) (snd ab0). rewrite mem_mgr_split. unfold KAF_globals, type_kalloc_token. rewrite mem_mgr_split. entailer!.
                 do 4 right. left; split; auto.
-- if_tac_auto_contradict. unfold KF_globals. rewrite kalloc_token_sz_split. unfold type_kalloc_token. rewrite kalloc_token_sz_split. entailer!.
+- if_tac_auto_contradict. unfold KAF_globals. rewrite kalloc_token_sz_split. unfold type_kalloc_token. rewrite kalloc_token_sz_split. entailer!.
 - if_tac_auto_contradict.
-    forward_call (kalloc_spec_sub KF_APD t_run) (gv, sh , original_freelist_pointer::ls, xx, pa1). (* kalloc *)
+    forward_call (kalloc_spec_sub KAF_APD t_run) (gv, sh , original_freelist_pointer::ls, xx, pa1). (* kalloc *)
     if_tac_auto_contradict.
     Intros ab.
-    forward_call (kfree_spec_sub KF_APD t_run) (pa2, gv, sh , snd ab, xx, fst ab). (* call kfree *)
+    forward_call (kfree_spec_sub KAF_APD t_run) (pa2, gv, sh , snd ab, xx, fst ab). (* call kfree *)
     ++ entailer!.
-    ++ if_tac_auto_contradict. forward_call (kalloc_spec_sub KF_APD t_run) (gv, sh , snd ab, xx, fst ab). (* kalloc *)
+    ++ if_tac_auto_contradict. forward_call (kalloc_spec_sub KAF_APD t_run) (gv, sh , snd ab, xx, fst ab). (* kalloc *)
         forward. if_tac_auto_contradict; inversion H5.
         ** Exists (fst ab). if_tac_auto_contradict.
-        unfold type_kalloc_token, KF_globals. entailer!.
+        unfold type_kalloc_token, KAF_globals. entailer!.
         do 2 right; left; split; auto.
         ** Intros ab0. Exists (fst ab). if_tac_auto_contradict.
-            Exists (fst ab0) (snd ab0). unfold type_kalloc_token, KF_globals. entailer!.
+            Exists (fst ab0) (snd ab0). unfold type_kalloc_token, KAF_globals. entailer!.
             do 3 right; left; split; auto.
-- if_tac_auto_contradict. unfold KF_globals. unfold type_kalloc_token. entailer!.
-- if_tac_auto_contradict. forward_call (kalloc_spec_sub KF_APD t_run) (gv, sh , original_freelist_pointer::ls, xx, pa1). (* kalloc *)
+- if_tac_auto_contradict. unfold KAF_globals. unfold type_kalloc_token. entailer!.
+- if_tac_auto_contradict. forward_call (kalloc_spec_sub KAF_APD t_run) (gv, sh , original_freelist_pointer::ls, xx, pa1). (* kalloc *)
     if_tac_auto_contradict.
     Intros ab.
-    forward_call (kfree_spec_sub KF_APD t_run) (pa2, gv, sh , snd ab, xx, fst ab). (* call kfree *)
+    forward_call (kfree_spec_sub KAF_APD t_run) (pa2, gv, sh , snd ab, xx, fst ab). (* call kfree *)
     + if_tac_auto_contradict. unfold type_kalloc_token at 2; entailer!.
     + if_tac_auto_contradict.
-    forward_call (kalloc_spec_sub KF_APD t_run) (gv, sh , fst ab::snd ab, xx, pa2). (* kalloc *)
+    forward_call (kalloc_spec_sub KAF_APD t_run) (gv, sh , fst ab::snd ab, xx, pa2). (* kalloc *)
     if_tac_auto_contradict.
-    Intros ab0. forward. Exists pa2. unfold KF_globals. unfold type_kalloc_token; entailer!.
+    Intros ab0. forward. Exists pa2. unfold KAF_globals. unfold type_kalloc_token; entailer!.
     inversion H8. rewrite H14, H15. inversion H5. rewrite H16, H17. entailer!.
         Qed.
         
-Lemma body_kfree_kfree_kalloc: semax_body KFVprog KFGprog f_kfree_kfree_kalloc kfree_kfree_kalloc_spec.
+Lemma body_kfree_kfree_kalloc: semax_body KAFVprog KAFGprog f_kfree_kfree_kalloc kfree_kfree_kalloc_spec.
 Proof.
 start_function.
 Intros.
 if_tac; if_tac; destruct H; 
-forward_call (kfree_spec_sub KF_APD t_run) (pa1, gv, sh , ls, xx, original_freelist_pointer). (* call kfree *)
-- if_tac_auto_contradict. unfold KF_globals. entailer!.
+forward_call (kfree_spec_sub KAF_APD t_run) (pa1, gv, sh , ls, xx, original_freelist_pointer). (* call kfree *)
+- if_tac_auto_contradict. unfold KAF_globals. entailer!.
 - if_tac_auto_contradict;
-    forward_call (kfree_spec_sub KF_APD t_run) (pa2, gv, sh , ls, xx, original_freelist_pointer). (* call kfree*)
+    forward_call (kfree_spec_sub KAF_APD t_run) (pa2, gv, sh , ls, xx, original_freelist_pointer). (* call kfree*)
     + if_tac_auto_contradict. entailer!.
     + if_tac_auto_contradict.
-        forward_call (kalloc_spec_sub KF_APD t_run) (gv, sh , ls, xx, original_freelist_pointer). (* kalloc *)
+        forward_call (kalloc_spec_sub KAF_APD t_run) (gv, sh , ls, xx, original_freelist_pointer). (* kalloc *)
         if_tac_auto_contradict. 
-        * forward. Exists nullval. unfold KF_globals. entailer!.
+        * forward. Exists nullval. unfold KAF_globals. entailer!.
         * forward. Exists original_freelist_pointer. Exists (fst ab) (snd ab). entailer!. 
-        unfold type_kalloc_token, KF_globals. entailer!.
--if_tac_auto_contradict. unfold KF_globals. entailer!.
+        unfold type_kalloc_token, KAF_globals. entailer!.
+-if_tac_auto_contradict. unfold KAF_globals. entailer!.
 -if_tac_auto_contradict;
-forward_call (kfree_spec_sub KF_APD t_run) (pa2, gv, sh , ls, xx,original_freelist_pointer). (* call kfree*)
+forward_call (kfree_spec_sub KAF_APD t_run) (pa2, gv, sh , ls, xx,original_freelist_pointer). (* call kfree*)
 + if_tac_auto_contradict. entailer!. unfold type_kalloc_token; entailer!. 
 + if_tac_auto_contradict.
-    forward_call (kalloc_spec_sub KF_APD t_run) (gv, sh , original_freelist_pointer::ls, xx, pa2). (* kalloc *)
+    forward_call (kalloc_spec_sub KAF_APD t_run) (gv, sh , original_freelist_pointer::ls, xx, pa2). (* kalloc *)
     if_tac_auto_contradict. 
-    forward. Exists pa2. unfold KF_globals. entailer!.
+    forward. Exists pa2. unfold KAF_globals. entailer!.
         * do 3 right. split; auto.
         * unfold type_kalloc_token. entailer!. inversion H0. rewrite H9, H10. entailer.
-- if_tac_auto_contradict. unfold KF_globals, type_kalloc_token. entailer!.
+- if_tac_auto_contradict. unfold KAF_globals, type_kalloc_token. entailer!.
 - if_tac_auto_contradict. 
-forward_call (kfree_spec_sub KF_APD t_run) (pa2, gv, sh , original_freelist_pointer::ls, xx,pa1). (* call kfree*)
+forward_call (kfree_spec_sub KAF_APD t_run) (pa2, gv, sh , original_freelist_pointer::ls, xx,pa1). (* call kfree*)
 + if_tac_auto_contradict. entailer!.
-+ if_tac_auto_contradict. forward_call (kalloc_spec_sub KF_APD t_run) (gv, sh , original_freelist_pointer::ls, xx, pa1). (* kalloc *)
++ if_tac_auto_contradict. forward_call (kalloc_spec_sub KAF_APD t_run) (gv, sh , original_freelist_pointer::ls, xx, pa1). (* kalloc *)
     if_tac_auto_contradict.
-    Intros ab. forward. Exists pa1. unfold type_kalloc_token, KF_globals. entailer!.
+    Intros ab. forward. Exists pa1. unfold type_kalloc_token, KAF_globals. entailer!.
     * do 2 right; left; split; auto.
     * inversion H6. rewrite H9, H10. entailer.
-- if_tac_auto_contradict. unfold type_kalloc_token, KF_globals. entailer!.
-- if_tac_auto_contradict. forward_call (kfree_spec_sub KF_APD t_run) (pa2, gv, sh , original_freelist_pointer::ls, xx,pa1). (* call kfree*)
+- if_tac_auto_contradict. unfold type_kalloc_token, KAF_globals. entailer!.
+- if_tac_auto_contradict. forward_call (kfree_spec_sub KAF_APD t_run) (pa2, gv, sh , original_freelist_pointer::ls, xx,pa1). (* call kfree*)
     + if_tac_auto_contradict. unfold type_kalloc_token. entailer!.
-    + if_tac_auto_contradict. forward_call (kalloc_spec_sub KF_APD t_run) (gv, sh , pa1::original_freelist_pointer::ls, xx, pa2). (* kalloc *)
+    + if_tac_auto_contradict. forward_call (kalloc_spec_sub KAF_APD t_run) (gv, sh , pa1::original_freelist_pointer::ls, xx, pa2). (* kalloc *)
     if_tac_auto_contradict. Intros ab.
-    forward. Exists pa2. unfold KF_globals, type_kalloc_token. entailer!.
+    forward. Exists pa2. unfold KAF_globals, type_kalloc_token. entailer!.
     inversion H6.
     entailer.
         Qed.
         
 
-Lemma body_kalloc_write_42_kfree_kfree: semax_body KFVprog KFGprog f_kalloc_write_42_kfree_kfree kalloc_write_42_kfree_kfree_spec.
+Lemma body_kalloc_write_42_kfree_kfree: semax_body KAFVprog KAFGprog f_kalloc_write_42_kfree_kfree kalloc_write_42_kfree_kfree_spec.
 Proof.
     start_function.
     forward. 
-    forward_call (kalloc_spec_sub KF_APD tint) (gv, sh , ls, xx, original_freelist_pointer ). (* kalloc *)
-    - unfold KF_globals. entailer!.
+    forward_call (kalloc_spec_sub KAF_APD tint) (gv, sh , ls, xx, original_freelist_pointer ). (* kalloc *)
+    - unfold KAF_globals. entailer!.
     - if_tac.
     + forward_if.
         * rewrite H in H0; auto_contradict.
-        * forward_call (kfree_spec_sub KF_APD t_run) (original_freelist_pointer, gv, sh , ls, xx,original_freelist_pointer). (* call kfree*)
+        * forward_call (kfree_spec_sub KAF_APD t_run) (original_freelist_pointer, gv, sh , ls, xx,original_freelist_pointer). (* call kfree*)
             -- if_tac_auto_contradict. entailer!.
             -- rewrite H. simpl. auto.
             -- if_tac_auto_contradict. 
@@ -605,41 +625,59 @@ Proof.
         * unfold type_kalloc_token. rewrite kalloc_token_sz_split. Intros.
         rewrite memory_block_data_at_; auto. rewrite data_at__eq. Intros. forward.
         forward. 
-        forward_call (kfree_spec_sub KF_APD tint) (original_freelist_pointer, gv, sh , snd ab, xx, (fst ab)). (* call kfree *)
+        forward_call (kfree_spec_sub KAF_APD tint) (original_freelist_pointer, gv, sh , snd ab, xx, (fst ab)). (* call kfree *)
         -- if_tac_auto_contradict.
             unfold type_kalloc_token. rewrite kalloc_token_sz_split. entailer!.
             sep_apply data_at_memory_block. entailer!.
         -- if_tac_auto_contradict.
             forward. Exists (Vint (Int.repr 42)).
-            unfold KF_globals.
+            unfold KAF_globals.
             inversion H0. rewrite H8; rewrite H9.
             entailer!.
         * rewrite H1 in H. auto_contradict.
         Qed.
 
 
-Lemma body_kfree_kfree_kalloc_kalloc: semax_body KFVprog KFGprog f_kfree_kfree_kalloc_kalloc kfree_kfree_kalloc_kalloc_spec.
+Lemma body_kfree_kfree_kalloc_kalloc: semax_body KAFVprog KAFGprog f_kfree_kfree_kalloc_kalloc kfree_kfree_kalloc_kalloc_spec.
 Proof.
 start_function.
 Intros.
 destruct H. 
-forward_call (kfree_spec_sub KF_APD t_run) (pa1, gv, sh , ls, xx, original_freelist_pointer). (* call kfree *)
-- unfold KF_globals.
+forward_call (kfree_spec_sub KAF_APD t_run) (pa1, gv, sh , ls, xx, original_freelist_pointer). (* call kfree *)
+- unfold KAF_globals.
     if_tac.
     + rewrite H1 in H. auto_contradict.
     + unfold type_kalloc_token. entailer!. 
 - if_tac_auto_contradict. rewrite H1 in H. auto_contradict.
-    forward_call (kfree_spec_sub KF_APD t_run) (pa2, gv, sh , original_freelist_pointer::ls, xx, pa1).
+    forward_call (kfree_spec_sub KAF_APD t_run) (pa2, gv, sh , original_freelist_pointer::ls, xx, pa1).
     if_tac_auto_contradict. rewrite H2 in H0; auto_contradict.
     unfold type_kalloc_token.
     entailer!.
-    forward_call (kalloc_spec_sub KF_APD t_run) (gv, sh , pa1::original_freelist_pointer::ls, xx, pa2). (* kalloc *)
+    forward_call (kalloc_spec_sub KAF_APD t_run) (gv, sh , pa1::original_freelist_pointer::ls, xx, pa2). (* kalloc *)
     if_tac_auto_contradict; entailer!.
     if_tac_auto_contradict. rewrite H2 in H0; auto_contradict.
     Intros ab. 
-    forward_call (kalloc_spec_sub KF_APD t_run) (gv, sh , original_freelist_pointer::ls, xx, pa1). (* kalloc *)
+    forward_call (kalloc_spec_sub KAF_APD t_run) (gv, sh , original_freelist_pointer::ls, xx, pa1). (* kalloc *)
     inversion H3. entailer!.
     if_tac_auto_contradict.
     Intros ab0. 
-    forward. unfold type_kalloc_token. entailer!. unfold KF_globals. inversion H5; entailer.
+    forward. unfold type_kalloc_token. entailer!. unfold KAF_globals. inversion H5; entailer.
+Qed.
+
+Lemma body_kfree_kfree_same_wrong_pointer: semax_body KAFVprog KAFGprog f_kfree_kfree_same_pointer kfree_kfree_same_pointer_wrong_spec.
+Proof.
+start_function.
+Intros.
+forward_call (kfree_spec_sub KAF_APD t_run) (pa1, gv, sh , ls, xx, original_freelist_pointer). (* call kfree *)
+- unfold KAF_globals.
+    if_tac.
+    + rewrite H0 in H. auto_contradict.
+    + unfold type_kalloc_token. entailer!. 
+- if_tac_auto_contradict. rewrite H0 in H. auto_contradict.
+    forward_call (kfree_spec_sub KAF_APD t_run) (pa1, gv, sh , original_freelist_pointer::ls, xx, pa1).
+    +  if_tac_auto_contradict. (*rewrite H2 in H0; auto_contradict.*)
+    unfold type_kalloc_token.
+    entailer!.
+    + if_tac_auto_contradict.
+      entailer. 
 Qed.
